\documentclass[12pt]{article}
\usepackage{pmmeta}
\pmcanonicalname{NonmodularSublattice}
\pmcreated{2013-03-22 16:55:25}
\pmmodified{2013-03-22 16:55:25}
\pmowner{ixionid}{16766}
\pmmodifier{ixionid}{16766}
\pmtitle{nonmodular sublattice}
\pmrecord{8}{39186}
\pmprivacy{1}
\pmauthor{ixionid}{16766}
\pmtype{Theorem}
\pmcomment{trigger rebuild}
\pmclassification{msc}{06C05}
%\pmkeywords{modular lattice sublattice}
\pmrelated{ModularLattice}

% this is the default PlanetMath preamble.  as your knowledge
% of TeX increases, you will probably want to edit this, but
% it should be fine as is for beginners.

% almost certainly you want these
\usepackage{amssymb}
\usepackage{amsmath}
\usepackage{amsfonts}

% used for TeXing text within eps files
%\usepackage{psfrag}
% need this for including graphics (\includegraphics)
%\usepackage{graphicx}
% for neatly defining theorems and propositions
\usepackage{amsthm}
% making logically defined graphics
%%\usepackage{xypic}

% there are many more packages, add them here as you need them

% define commands here

\begin{document}
Any nonmodular lattice $L$ contains the lattice $N_5$ (shown below) as a sublattice.
$$ \xymatrix {
& x\lor y \ar@{-}[ld] \ar@{-}[rdrd] & & \\
(x\lor y)\land z \ar@{-}[dd] & & & \\
& & & y \ar@{-}[ldld] \\
x\lor (y\land z) \ar@{-}[rd] & & & \\
& y\land z & & }  $$

\begin{proof}
Since $L$ is not modular, by definition it contains elements $x$, $y$ and $z$ such that $x\leq z$ and $x\lor (y\land z) < (x\lor y) \land z$.  Then the sublattice formed by $y$, $x\lor y$, $y\land z$, $(x\lor y)\land z$ and $x\lor (y\land z)$ is isomorphic to $N_5$.  This is because $y\land z\leq x\lor(y\land z)<(x\lor y)\land z\leq x\lor y$ while $[x\lor(y\land z)]\lor y=x\lor y$ by absorption and similarly $y\land[(x\lor y)\land z]=y\land z$. Moreover, $x\lor(y\land z)$ covers $y\land z$ since $y\land z=x\lor(y\land z)$ would imply $x\leq y\land z \leq y$, whence $x\lor y=y$ and $(x\lor y)\land z=y\land z=x\lor(y\land z)$ contrary to our hypothesis. By the same method, $ (x\lor y)\land z=x\lor y $ leads to a contradiction of nonmodularity, so $ x\lor y $ covers $ (x\lor y)\land z $.
\end{proof}
%%%%%
%%%%%
\end{document}
